updates for proofs of refinement

src/proofs/no_slashable_blocks/common/dvc_block_proposer_instrumented.dfy
@@ -14,14 +14,14 @@ module DVC_Block_Proposer_Spec_Instr {
 
 
     datatype BlockConsensusEngineState = BlockConsensusEngineState(
-        active_block_consensus_instances: map<Slot, BlockConsensusValidityCheckState>,
+        active_consensus_instances_on_beacon_blocks: map<Slot, BlockConsensusValidityCheckState>,
         ghost block_slashing_db_hist: map<Slot, map<BeaconBlock -> bool, set<set<SlashingDBBlock>>>>
     )
 
     function getInitialBlockConensusEngineState(): BlockConsensusEngineState
     {
         BlockConsensusEngineState(
-            active_block_consensus_instances := map[],
+            active_consensus_instances_on_beacon_blocks := map[],
             block_slashing_db_hist := map[]
         )
     }
@@ -33,7 +33,7 @@ module DVC_Block_Proposer_Spec_Instr {
         block_slashing_db: set<SlashingDBBlock>,
         complete_signed_randao_reveal: BLSSignature
     ): BlockConsensusEngineState
-    requires slot !in s.active_block_consensus_instances.Keys    
+    requires slot !in s.active_consensus_instances_on_beacon_blocks.Keys    
     requires slot == proposer_duty.slot
     {
         var bcvc := 
@@ -53,13 +53,13 @@ module DVC_Block_Proposer_Spec_Instr {
                                                                     bcvc.proposer_duty,
                                                                     bcvc.complete_signed_randao_reveal)));                
         
-        var new_active_block_consensus_instances := 
-            s.active_block_consensus_instances[
+        var new_active_consensus_instances_on_beacon_blocks := 
+            s.active_consensus_instances_on_beacon_blocks[
                 slot := bcvc
             ];
 
         s.(
-            active_block_consensus_instances := new_active_block_consensus_instances,
+            active_consensus_instances_on_beacon_blocks := new_active_consensus_instances_on_beacon_blocks,
             block_slashing_db_hist := 
                 addToBlockSlashingDBHist(
                     s.block_slashing_db_hist,
@@ -109,22 +109,22 @@ module DVC_Block_Proposer_Spec_Instr {
     ): BlockConsensusEngineState
     {
         s.(
-            active_block_consensus_instances := s.active_block_consensus_instances - ids
+            active_consensus_instances_on_beacon_blocks := s.active_consensus_instances_on_beacon_blocks - ids
         )
     }    
  
     function updateBlockSlashingDBHist(
         hist: map<Slot, map<BeaconBlock -> bool, set<set<SlashingDBBlock>>>>,
-        new_active_block_consensus_instances : map<Slot, BlockConsensusValidityCheckState>,
+        new_active_consensus_instances_on_beacon_blocks : map<Slot, BlockConsensusValidityCheckState>,
         new_block_slashing_db: set<SlashingDBBlock>
     ): (new_hist: map<Slot, map<BeaconBlock -> bool, set<set<SlashingDBBlock>>>>)
-    ensures hist.Keys + new_active_block_consensus_instances.Keys == new_hist.Keys
+    ensures hist.Keys + new_active_consensus_instances_on_beacon_blocks.Keys == new_hist.Keys
     {
             var ret 
-                := map k: Slot | k in (new_active_block_consensus_instances.Keys + hist.Keys)
+                := map k: Slot | k in (new_active_consensus_instances_on_beacon_blocks.Keys + hist.Keys)
                     ::            
-                    if k in new_active_block_consensus_instances.Keys then 
-                        var vp := new_active_block_consensus_instances[k].validityPredicate;
+                    if k in new_active_consensus_instances_on_beacon_blocks.Keys then 
+                        var vp := new_active_consensus_instances_on_beacon_blocks[k].validityPredicate;
                         var hist_k := getOrDefault(hist, k, map[]);
                         var hist_k_vp := getOrDefault(hist_k, vp, {}) + {new_block_slashing_db};
                         hist_k[
@@ -158,36 +158,33 @@ module DVC_Block_Proposer_Spec_Instr {
         new_block_slashing_db: set<SlashingDBBlock>
     ): (r: BlockConsensusEngineState)
     {
-        var new_active_block_consensus_instances := updateBlockConsensusInstanceValidityCheckHelper(
-                    s.active_block_consensus_instances,
+        var new_active_consensus_instances_on_beacon_blocks := updateBlockConsensusInstanceValidityCheckHelper(
+                    s.active_consensus_instances_on_beacon_blocks,
                     new_block_slashing_db
                 );
         s.(
-            active_block_consensus_instances := new_active_block_consensus_instances,
+            active_consensus_instances_on_beacon_blocks := new_active_consensus_instances_on_beacon_blocks,
             block_slashing_db_hist := updateBlockSlashingDBHist(
                 s.block_slashing_db_hist,
-                new_active_block_consensus_instances,
+                new_active_consensus_instances_on_beacon_blocks,
                 new_block_slashing_db
             )
         )
     }
 
-
     datatype DVCState = DVCState(
         current_proposer_duty: Optional<ProposerDuty>,
-        last_served_proposer_duty: Optional<ProposerDuty>,
+        latest_proposer_duty: Optional<ProposerDuty>,
         block_slashing_db: set<SlashingDBBlock>,
-        block_share_db: BlockSignatureShareDB,        
         rcvd_randao_shares: map<Slot, set<RandaoShare>>,
-        rcvd_block_shares: map<Slot, map<BeaconBlock, set<SignedBeaconBlock>>>,
-        construct_signed_randao_reveal: (set<BLSSignature>) -> Optional<BLSSignature>,
-        construct_signed_block: (set<SignedBeaconBlock>) -> Optional<SignedBeaconBlock>,
-        block_shares_to_broadcast: map<Slot, SignedBeaconBlock>, 
+        rcvd_signed_beacon_blocks: map<Slot, map<BeaconBlock, set<SignedBeaconBlock>>>,
+        construct_complete_signed_randao_reveal: (set<BLSSignature>) -> Optional<BLSSignature>,
+        construct_complete_signed_block: (set<SignedBeaconBlock>) -> Optional<SignedBeaconBlock>,
+        signed_beacon_blocks_to_broadcast: map<Slot, SignedBeaconBlock>, 
         randao_shares_to_broadcast: map<Slot, RandaoShare>,
         peers: set<BLSPubkey>,        
-        // TODO: Note difference with spec.py
         dv_pubkey: BLSPubkey,
-        future_decided_slots: map<Slot, BeaconBlock>,
+        future_consensus_instances_on_blocks_already_decided: map<Slot, BeaconBlock>,
         bn: BNState,
         rs: RSState,
         block_consensus_engine_state: BlockConsensusEngineState,
@@ -215,7 +212,7 @@ module DVC_Block_Proposer_Spec_Instr {
     {
         var setWithRecipient := set m | m in ms :: addRecepientsToMessage(m, receipients);
         setUnion(setWithRecipient)
-    }    
+    }
 
     datatype DVCStateAndOuputs = DVCStateAndOuputs(
         state: DVCState,
@@ -226,82 +223,91 @@ module DVC_Block_Proposer_Spec_Instr {
         s: DVCState,         
         dv_pubkey: BLSPubkey,
         peers: set<BLSPubkey>,                    
-        construct_signed_randao_reveal: (set<BLSSignature>) -> Optional<BLSSignature>,
-        construct_signed_block: (set<SignedBeaconBlock>) -> Optional<SignedBeaconBlock>,        
+        construct_complete_signed_randao_reveal: (set<BLSSignature>) -> Optional<BLSSignature>,
+        construct_complete_signed_block: (set<SignedBeaconBlock>) -> Optional<SignedBeaconBlock>,        
         initial_block_slashing_db: set<SlashingDBBlock>,
         rs_pubkey: BLSPubkey
     )
+    requires && s.bn.state_roots_of_imported_blocks == {}
+             && s.bn.blocks_submitted == []
     {
         s == DVCState(
             // proposer_duty_queue := [],
-            future_decided_slots := map[],
-            block_shares_to_broadcast := map[],
+            future_consensus_instances_on_blocks_already_decided := map[],
+            signed_beacon_blocks_to_broadcast := map[],
             randao_shares_to_broadcast := map[],
             block_slashing_db := initial_block_slashing_db,
-            block_share_db := map[],
             rcvd_randao_shares := map[],
-            rcvd_block_shares := map[],
+            rcvd_signed_beacon_blocks := map[],
             current_proposer_duty := None,
-            last_served_proposer_duty := None,
+            latest_proposer_duty := None,
             bn := s.bn,
             rs := DVC_Block_Proposer_Spec_NonInstr.getInitialRS(rs_pubkey),
             dv_pubkey := dv_pubkey,
             peers := peers,                        
-            construct_signed_block := construct_signed_block,
-            construct_signed_randao_reveal := construct_signed_randao_reveal,
+            construct_complete_signed_block := construct_complete_signed_block,
+            construct_complete_signed_randao_reveal := construct_complete_signed_randao_reveal,
             block_consensus_engine_state := getInitialBlockConensusEngineState(),
             all_rcvd_duties := {}
         )
     }
 
-    // predicate Next(
-    //     s: DVCState,
-    //     event: Event,
-    //     s': DVCState,
-    //     outputs: Outputs
-    // )
-    // {
-    //     var newNodeStateAndOutputs := DVCStateAndOuputs(
-    //         state := s',
-    //         outputs := outputs
-    //     );
+    predicate Next(
+        s: DVCState,
+        event: Event,
+        s': DVCState,
+        outputs: Outputs
+    )
+    {
+        &&  var newNodeStateAndOutputs := 
+                DVCStateAndOuputs(
+                    state := s',
+                    outputs := outputs
+                );
+        && f_process_event.requires(s, event)
+        && newNodeStateAndOutputs == f_process_event(s, event)
+    }
 
-    //     newNodeStateAndOutputs == f_process_event(s, event)
-    // }
-
-    // function f_process_event(
-    //     s: DVCState,
-    //     event: Event
-    // ): DVCStateAndOuputs
-    // requires
-    //         match event 
-    //         case ServeAttstationDuty(proposer_duty) => 
-    //             && f_serve_proposer_duty.requires(s, proposer_duty)
-    //         case AttConsensusDecided(id, decided_block_data) => 
-    //             && f_block_consensus_decided.requires(s, id,  decided_block_data)
-    //         case ReceivedAttestationShare(block_share) => 
-    //             f_listen_for_block_shares.requires(s, block_share)
-    //         case ImportedNewBlock(block) => 
-    //             f_listen_for_new_imported_blocks.requires(s, block)
-    //         case ResendAttestationShares => 
-    //             f_resend_block_share.requires(s) 
-    //         case NoEvent => 
-    //             true
-    // {
-    //     match event 
-    //         case ServeAttstationDuty(proposer_duty) => 
-    //             f_serve_proposer_duty(s, proposer_duty)
-    //         case AttConsensusDecided(id, decided_block_data) => 
-    //             f_block_consensus_decided(s, id,  decided_block_data)
-    //         case ReceivedAttestationShare(block_share) => 
-    //             f_listen_for_block_shares(s, block_share)
-    //         case ImportedNewBlock(block) => 
-    //             f_listen_for_new_imported_blocks(s, block)
-    //         case ResendAttestationShares => 
-    //             f_resend_block_share(s)
-    //         case NoEvent => 
-    //             DVCStateAndOuputs(state := s, outputs := getEmptyOuputs() )
-    // }  
+    function f_process_event(
+        s: DVCState,
+        event: Event        
+    ): DVCStateAndOuputs
+    requires match event         
+                case ServeProposerDuty(proposer_duty) => 
+                    && f_serve_proposer_duty.requires(s, proposer_duty)
+                case BlockConsensusDecided(id, block) => 
+                    && f_block_consensus_decided.requires(s, id, block)
+                case ReceiveRandaoShare(randao_share) => 
+                    && f_listen_for_randao_shares.requires(s, randao_share)
+                case ReceiveSignedBeaconBlock(block_share) => 
+                    && f_listen_for_block_signature_shares.requires(s, block_share)
+                case ImportedNewBlock(block) => 
+                    && f_listen_for_new_imported_blocks.requires(s, block)
+                case ResendRandaoRevealSignatureShare => 
+                    && f_resend_randao_share.requires(s)
+                case ResendBlockShare => 
+                    && f_resend_block_share.requires(s) 
+                case NoEvent => 
+                    true
+    {
+        match event         
+            case ServeProposerDuty(proposer_duty) => 
+                f_serve_proposer_duty(s, proposer_duty)
+            case BlockConsensusDecided(id, block) => 
+                f_block_consensus_decided(s, id, block)
+            case ReceiveRandaoShare(randao_share) => 
+                f_listen_for_randao_shares(s, randao_share)
+            case ReceiveSignedBeaconBlock(block_share) => 
+                f_listen_for_block_signature_shares(s, block_share)
+            case ImportedNewBlock(block) => 
+                f_listen_for_new_imported_blocks(s, block)
+            case ResendRandaoRevealSignatureShare => 
+                f_resend_randao_share(s)
+            case ResendBlockShare => 
+                f_resend_block_share(s) 
+            case NoEvent => 
+                DVCStateAndOuputs(state := s, outputs := getEmptyOuputs() )
+    }
 
     function merge_two_outputs(
         outputs1: Outputs,
@@ -310,12 +316,11 @@ module DVC_Block_Proposer_Spec_Instr {
     {
         getEmptyOuputs().(
             block_shares_sent := outputs1.block_shares_sent + outputs2.block_shares_sent,
-            randao_shares_sent := outputs1.randao_shares_sent + outputs2.randao_shares_sent,
+            sent_randao_shares := outputs1.sent_randao_shares + outputs2.sent_randao_shares,
             submitted_signed_blocks := outputs1.submitted_signed_blocks + outputs2.submitted_signed_blocks
         )
-    }  
+    }
 
-    // Wraps a DVC state with outputs to construct a state with type DVCStateAndOutputs
     function f_wrap_DVCState_with_Outputs(
         dvc: DVCState,
         outputs: Outputs
@@ -326,7 +331,7 @@ module DVC_Block_Proposer_Spec_Instr {
                 state := dvc,
                 outputs := outputs
             )
-    }  
+    }
 
     function f_terminate_current_proposer_duty(
         process: DVCState
@@ -346,7 +351,7 @@ module DVC_Block_Proposer_Spec_Instr {
         // or it knew a decision for the last proposer duty.
         else 
             process
-    }  
+    }
 
     function f_serve_proposer_duty(
         process: DVCState,
@@ -367,26 +372,32 @@ module DVC_Block_Proposer_Spec_Instr {
 
     function f_broadcast_randao_share(
         process: DVCState,
-        serving_duty: ProposerDuty
+        proposer_duty: ProposerDuty
     ): DVCStateAndOuputs 
     {
-        var slot := serving_duty.slot;
-        var epoch := compute_epoch_at_slot(slot);            
+        var slot := proposer_duty.slot;
         var fork_version := bn_get_fork_version(slot);    
-        var root := compute_randao_reveal_signing_root(slot);
-        var randao_signature := rs_sign_randao_reveal(slot, fork_version, root, process.rs);                                                           
-        var randao_share := RandaoShare(serving_duty, epoch, slot, root, randao_signature);        
+        var epoch := compute_epoch_at_slot(slot);
+        var randao_reveal_signing_root := compute_randao_reveal_signing_root(slot);
+        var randao_reveal_signature_share := rs_sign_randao_reveal(epoch, fork_version, randao_reveal_signing_root, process.rs);
+        var randao_share := 
+            RandaoShare(
+                proposer_duty := proposer_duty,
+                slot := slot,
+                signing_root := randao_reveal_signing_root,
+                signature_share := randao_reveal_signature_share
+            );
         var broadcasted_output := 
             getEmptyOuputs().(
-                randao_shares_sent := multicast(randao_share, process.peers)                                            
+                sent_randao_shares := multicast(randao_share, process.peers)                                            
             );
         
         var process_after_checking_for_next_duty := 
             f_check_for_next_duty(
                 process.(
-                    randao_shares_to_broadcast := process.randao_shares_to_broadcast[serving_duty.slot := randao_share]
+                    randao_shares_to_broadcast := process.randao_shares_to_broadcast[proposer_duty.slot := randao_share]
                 ),
-                serving_duty
+                proposer_duty
             );
         
         var merged_outputs := merge_two_outputs(broadcasted_output, process_after_checking_for_next_duty.outputs);
@@ -396,37 +407,70 @@ module DVC_Block_Proposer_Spec_Instr {
             merged_outputs
         )
     }
-  
+
     function f_check_for_next_duty(
         process: DVCState,
-        serving_duty: ProposerDuty
+        proposer_duty: ProposerDuty
     ): DVCStateAndOuputs 
     {            
-        var slot := serving_duty.slot;
-        if slot in process.future_decided_slots 
+        var slot := proposer_duty.slot;
+        if slot in process.future_consensus_instances_on_blocks_already_decided 
         then        
-            var block := process.future_decided_slots[slot];                
-            var process_with_updated_slashing_db := f_update_block_slashing_db(process, block);            
-            var process_after_removing_slot
+            var block := process.future_consensus_instances_on_blocks_already_decided[slot];                
+            var new_block_slashing_db := 
+                f_update_block_slashing_db(process.block_slashing_db, block);            
+            var new_process
                 := 
-                process_with_updated_slashing_db.(                        
-                    future_decided_slots := process.future_decided_slots - {slot}
+                process.(
+                    current_proposer_duty := None,
+                    latest_proposer_duty := Some(proposer_duty),
+                    future_consensus_instances_on_blocks_already_decided := process.future_consensus_instances_on_blocks_already_decided - {slot},
+                    block_slashing_db := new_block_slashing_db,
+                    block_consensus_engine_state := updateBlockConsensusInstanceValidityCheck(
+                            process.block_consensus_engine_state,
+                            new_block_slashing_db
+                    )     
                 );
 
             f_wrap_DVCState_with_Outputs(
-                process_after_removing_slot,
+                new_process,
                 getEmptyOuputs()
             )    
         else 
             var process_after_adding_new_duty := 
                 process.(
-                    current_proposer_duty := Some(serving_duty),
-                    last_served_proposer_duty := Some(serving_duty)
+                    current_proposer_duty := Some(proposer_duty),
+                    latest_proposer_duty := Some(proposer_duty)
                 );
 
             f_start_consensus_if_can_construct_randao_share(
                 process_after_adding_new_duty
             )                    
+    }
+
+    function f_listen_for_randao_shares(
+        process: DVCState,
+        randao_share: RandaoShare
+    ): DVCStateAndOuputs         
+    {
+        var slot := randao_share.slot;
+        var active_consensus_instances_on_beacon_blocks := process.block_consensus_engine_state.active_consensus_instances_on_beacon_blocks.Keys;
+
+        if is_slot_for_current_or_future_instances(process, slot) 
+        then
+            var process_with_dlv_randao_share := 
+                    process.(
+                        rcvd_randao_shares := process.rcvd_randao_shares[slot := getOrDefault(process.rcvd_randao_shares, slot, {}) + 
+                                                                                        {randao_share} ]
+                    );     
+            f_start_consensus_if_can_construct_randao_share(
+                process_with_dlv_randao_share
+            )
+        else
+            f_wrap_DVCState_with_Outputs(
+                process,
+                getEmptyOuputs()
+            )
     }
 
     function f_start_consensus_if_can_construct_randao_share(
@@ -440,10 +484,10 @@ module DVC_Block_Proposer_Spec_Instr {
             var all_rcvd_randao_sig := 
                     set randao_share | randao_share in process.rcvd_randao_shares[
                                                 process.current_proposer_duty.safe_get().slot]
-                                                    :: randao_share.signature;                
-            var constructed_randao_reveal := process.construct_signed_randao_reveal(all_rcvd_randao_sig);
+                                                    :: randao_share.signature_share;                
+            var constructed_randao_reveal := process.construct_complete_signed_randao_reveal(all_rcvd_randao_sig);
             if && constructed_randao_reveal.isPresent()  
-               && proposer_duty.slot !in process.block_consensus_engine_state.active_block_consensus_instances.Keys 
+               && proposer_duty.slot !in process.block_consensus_engine_state.active_consensus_instances_on_beacon_blocks.Keys 
             then                      
                 var validityPredicate := ((block: BeaconBlock)  => 
                                             consensus_is_valid_beacon_block(
@@ -476,34 +520,32 @@ module DVC_Block_Proposer_Spec_Instr {
     }
     
     function f_update_block_slashing_db(
-        process: DVCState,        
+        block_slashing_db: set<SlashingDBBlock>,
         block: BeaconBlock
-    ): DVCState
+    ): set<SlashingDBBlock>
     {   
-        var newDBBlock := SlashingDBBlock(block.slot, hash_tree_root(block));        
-        process.(                 
-            block_slashing_db := process.block_slashing_db + {newDBBlock}        
-        )
-    }       
-    
+        var new_slashingDB_block := SlashingDBBlock(block.slot, hash_tree_root(block));        
+        block_slashing_db + {new_slashingDB_block}                
+    }
+
     function f_block_consensus_decided(
         process: DVCState,
         id: Slot,
         block: BeaconBlock
     ): DVCStateAndOuputs
     {
-        if  && process.current_proposer_duty.isPresent()
-            && id == process.current_proposer_duty.safe_get().slot
-            && id == block.slot
+        if && process.current_proposer_duty.isPresent()
+           && process.current_proposer_duty.safe_get().slot == block.slot
+           && id == block.slot
         then
-            var process_with_updated_slashing_db := f_update_block_slashing_db(process, block);
+            var process_with_updated_slashing_db := f_update_block_slashing_db(process.block_slashing_db, block);
             var block_signing_root := compute_block_signing_root(block);
             var fork_version := bn_get_fork_version(block.slot);
             var block_signature := rs_sign_block(block, fork_version, block_signing_root, process.rs);
             var block_share := SignedBeaconBlock(block, block_signature);
             var slot := block.slot;
             var process_after_broadcasting_block_share := process.(                
-                    block_shares_to_broadcast := process.block_shares_to_broadcast[slot := block_share]
+                    signed_beacon_blocks_to_broadcast := process.signed_beacon_blocks_to_broadcast[slot := block_share]
                 );
             var multicastOutputs := getEmptyOuputs().(
                                         block_shares_sent := multicast(block_share, process.peers)
@@ -512,10 +554,13 @@ module DVC_Block_Proposer_Spec_Instr {
             f_wrap_DVCState_with_Outputs(
                 process_after_broadcasting_block_share,
                 merge_two_outputs(multicastOutputs, getEmptyOuputs())
-            )   
-        else 
-            f_wrap_DVCState_with_Outputs(process, getEmptyOuputs())               
-    }    
+            )
+        else
+            f_wrap_DVCState_with_Outputs(
+                process,
+                getEmptyOuputs()
+            )
+    }
 
     predicate is_slot_for_current_or_future_instances(
         process: DVCState,        
@@ -528,15 +573,15 @@ module DVC_Block_Proposer_Spec_Instr {
         // inconsistency should be fixed up by either accepting here only shares with slot higher than the
         // maximum already-decided slot or changing the clean-up code in listen_for_new_imported_blocks to clean
         // up only slot lower thant the slot of the current/latest duty.
-        var active_block_consensus_instances := 
-            process.block_consensus_engine_state.active_block_consensus_instances.Keys;
+        var active_consensus_instances_on_beacon_blocks := 
+            process.block_consensus_engine_state.active_consensus_instances_on_beacon_blocks.Keys;
 
-        || (active_block_consensus_instances == {} && !process.last_served_proposer_duty.isPresent())
-        || (active_block_consensus_instances != {} && get_min(active_block_consensus_instances) <= received_slot)
-        || (active_block_consensus_instances == {} && !process.current_proposer_duty.isPresent() && process.last_served_proposer_duty.isPresent() && process.last_served_proposer_duty.safe_get().slot < received_slot)            
+        || (active_consensus_instances_on_beacon_blocks == {} && !process.latest_proposer_duty.isPresent())
+        || (active_consensus_instances_on_beacon_blocks != {} && get_min(active_consensus_instances_on_beacon_blocks) <= received_slot)
+        || (active_consensus_instances_on_beacon_blocks == {} && !process.current_proposer_duty.isPresent() && process.latest_proposer_duty.isPresent() && process.latest_proposer_duty.safe_get().slot < received_slot)            
     }
 
-    function f_listen_for_block_share(
+    function f_listen_for_block_signature_shares(
         process: DVCState,
         block_share: SignedBeaconBlock
     ): DVCStateAndOuputs
@@ -545,21 +590,21 @@ module DVC_Block_Proposer_Spec_Instr {
 
         if is_slot_for_current_or_future_instances(process, slot) then
             var data := block_share.message;
-            var rcvd_block_shares_db_at_slot := getOrDefault(process.rcvd_block_shares, slot, map[]);
+            var rcvd_signed_beacon_blocks_db_at_slot := getOrDefault(process.rcvd_signed_beacon_blocks, slot, map[]);
             var process_with_new_block_share :=
                 process.(
-                    rcvd_block_shares := 
-                        process.rcvd_block_shares[
+                    rcvd_signed_beacon_blocks := 
+                        process.rcvd_signed_beacon_blocks[
                             slot := 
-                                rcvd_block_shares_db_at_slot[
+                                rcvd_signed_beacon_blocks_db_at_slot[
                                     data := 
-                                        getOrDefault(rcvd_block_shares_db_at_slot, data, {}) + 
+                                        getOrDefault(rcvd_signed_beacon_blocks_db_at_slot, data, {}) + 
                                         {block_share}
                                     ]
                         ]
                 );            
-            if process.construct_signed_block(process_with_new_block_share.rcvd_block_shares[slot][data]).isPresent() then                
-                    var complete_signed_block := process.construct_signed_block(process_with_new_block_share.rcvd_block_shares[slot][data]).safe_get();                      
+            if process.construct_complete_signed_block(process_with_new_block_share.rcvd_signed_beacon_blocks[slot][data]).isPresent() then                
+                    var complete_signed_block := process.construct_complete_signed_block(process_with_new_block_share.rcvd_signed_beacon_blocks[slot][data]).safe_get();                      
                     f_wrap_DVCState_with_Outputs(
                         process_with_new_block_share,
                         getEmptyOuputs().(
@@ -578,100 +623,91 @@ module DVC_Block_Proposer_Spec_Instr {
             )     
     }
 
-    function f_listen_for_randao_share(
-        process: DVCState,
-        randao_share: RandaoShare
-    ): DVCStateAndOuputs         
-    {
-        var slot := randao_share.slot;
-        var active_block_consensus_instances := process.block_consensus_engine_state.active_block_consensus_instances.Keys;
-
-        if is_slot_for_current_or_future_instances(process, slot) 
-        then
-            var process_with_dlv_randao_share := 
-                    process.(
-                        rcvd_randao_shares := process.rcvd_randao_shares[slot := getOrDefault(process.rcvd_randao_shares, slot, {}) + 
-                                                                                        {randao_share} ]
-                    );     
-            f_start_consensus_if_can_construct_randao_share(
-                process_with_dlv_randao_share
-            )
-        else
-            f_wrap_DVCState_with_Outputs(
-                process,
-                getEmptyOuputs()
-            )
-    }   
-
     
-    function f_listen_for_new_imported_block(
+    // How to prove that DVC_Block_Proposer_Spec_NonInstr.isMyAttestation is equivalent
+    // to DVC_Block_Proposer_Spec_Instr.isMyAttestation?
+    // predicate isMyAttestation(
+    //     a: Attestation,
+    //     bn: BNState,
+    //     block: BeaconBlock,
+    //     valIndex: Optional<ValidatorIndex>
+    // )
+    // requires block.body.state_root in bn.state_roots_of_imported_blocks
+    // {
+    //         && var committee := bn_get_epoch_committees(bn, block.body.state_root, a.data.index);
+    //         && valIndex.Some?
+    //         && valIndex.v in committee
+    //         && var i:nat :| i < |committee| && committee[i] == valIndex.v;
+    //         && i < |a.aggregation_bits|
+    //         && a.aggregation_bits[i]         
+    // }
+
+    function f_listen_for_new_imported_blocks_helper(
         process: DVCState,
-        signed_block: SignedBeaconBlock
-    ): DVCStateAndOuputs
-    {        
-        var block_consensus_already_decided := 
-            if verify_bls_signature(signed_block.message, signed_block.signature, process.dv_pubkey) then
-                process.future_decided_slots[
-                    signed_block.message.slot := signed_block.message
-                ]
-            else 
-                process.future_decided_slots
-            ;
-
-        var new_block_consensus_engine_state := stopBlockConsensusInstances(
-                                                    process.block_consensus_engine_state,
-                                                    block_consensus_already_decided.Keys
-                                                );
-
-        var cleaned_up_process := 
-            process.(
-                block_shares_to_broadcast := process.block_shares_to_broadcast - block_consensus_already_decided.Keys,
-                rcvd_block_shares := process.rcvd_block_shares - block_consensus_already_decided.Keys,
-                randao_shares_to_broadcast := process.randao_shares_to_broadcast - block_consensus_already_decided.Keys,
-                rcvd_randao_shares := process.rcvd_randao_shares - block_consensus_already_decided.Keys,
-                block_consensus_engine_state := new_block_consensus_engine_state
-            );
-
-        var process_with_new_future_decided_slots :=
-            if cleaned_up_process.last_served_proposer_duty.isPresent() then
-                var slot := cleaned_up_process.last_served_proposer_duty.safe_get().slot;
-                var old_instances := set i | 
-                                        && i in block_consensus_already_decided 
-                                        && i <= cleaned_up_process.last_served_proposer_duty.safe_get().slot;
-                cleaned_up_process.(
-                    future_decided_slots := block_consensus_already_decided - old_instances
-                )                      
-            else
-                cleaned_up_process.(
-                    future_decided_slots := block_consensus_already_decided
-                )
-            ;
-
-        if && process_with_new_future_decided_slots.current_proposer_duty.isPresent() 
-           && process_with_new_future_decided_slots.current_proposer_duty.safe_get().slot in block_consensus_already_decided.Keys
-        then
-            var process_with_new_slashing_db := 
-                f_update_block_slashing_db(
-                    process_with_new_future_decided_slots,
-                    block_consensus_already_decided[
-                        process_with_new_future_decided_slots.current_proposer_duty.safe_get().slot
-                    ]
-                );
-            var process_without_current_duty := process_with_new_future_decided_slots.(
-                                                current_proposer_duty := None
-                                            );
-            
-            f_wrap_DVCState_with_Outputs(
-                process_without_current_duty,
-                getEmptyOuputs()
-            )
+        consensus_instances_on_blocks_already_decided: map<Slot, BeaconBlock>
+    ): map<int, BeaconBlock>
+    {
+        if process.latest_proposer_duty.isPresent() then
+            var old_instances := 
+                    set i | 
+                        && i in consensus_instances_on_blocks_already_decided.Keys
+                        && i <= process.latest_proposer_duty.safe_get().slot
+                    ;
+            consensus_instances_on_blocks_already_decided - old_instances
         else
-            f_wrap_DVCState_with_Outputs(
-                process_with_new_future_decided_slots,
-                getEmptyOuputs()
-            )
+            consensus_instances_on_blocks_already_decided     
     }
-  
+
+    function f_listen_for_new_imported_blocks(
+        process: DVCState,
+        block: BeaconBlock
+    ): DVCStateAndOuputs
+    requires block.body.state_root in process.bn.state_roots_of_imported_blocks
+    requires    var valIndex := bn_get_validator_index(process.bn, block.body.state_root, process.dv_pubkey);
+                forall a1, a2 | 
+                        && a1 in block.body.attestations
+                        && DVC_Block_Proposer_Spec_NonInstr.isMyAttestation(a1, process.bn, block, valIndex)
+                        && a2 in block.body.attestations
+                        && DVC_Block_Proposer_Spec_NonInstr.isMyAttestation(a2, process.bn, block, valIndex)                        
+                    ::
+                        a1.data.slot == a2.data.slot ==> a1 == a2
+    {    
+        var new_consensus_instances_on_blocks_already_decided: map<Slot, BeaconBlock> := 
+            map[ block.slot := block ];
+
+        var consensus_instances_on_blocks_already_decided := process.future_consensus_instances_on_blocks_already_decided + new_consensus_instances_on_blocks_already_decided;
+
+        var future_consensus_instances_on_blocks_already_decided := 
+            f_listen_for_new_imported_blocks_helper(process, consensus_instances_on_blocks_already_decided);
+
+        var process_after_stopping_consensus_instance :=
+            process.(
+                future_consensus_instances_on_blocks_already_decided := future_consensus_instances_on_blocks_already_decided,
+                block_consensus_engine_state := stopBlockConsensusInstances(
+                                process.block_consensus_engine_state,
+                                consensus_instances_on_blocks_already_decided.Keys
+                ),
+                signed_beacon_blocks_to_broadcast := process.signed_beacon_blocks_to_broadcast - consensus_instances_on_blocks_already_decided.Keys,
+                rcvd_signed_beacon_blocks := process.rcvd_signed_beacon_blocks - consensus_instances_on_blocks_already_decided.Keys                    
+            );   
+
+        if process_after_stopping_consensus_instance.current_proposer_duty.isPresent() && process_after_stopping_consensus_instance.current_proposer_duty.safe_get().slot in consensus_instances_on_blocks_already_decided then
+            var decided_beacon_blocks := consensus_instances_on_blocks_already_decided[process.current_proposer_duty.safe_get().slot];
+            var new_block_slashing_db := f_update_block_slashing_db(process.block_slashing_db, decided_beacon_blocks);
+            var process_after_updating_validity_check := 
+                    process_after_stopping_consensus_instance.(
+                    current_proposer_duty := None,
+                    block_slashing_db := new_block_slashing_db,
+                    block_consensus_engine_state := updateBlockConsensusInstanceValidityCheck(
+                        process_after_stopping_consensus_instance.block_consensus_engine_state,
+                        new_block_slashing_db
+                    )                
+            );
+            f_wrap_DVCState_with_Outputs(process_after_updating_validity_check, getEmptyOuputs())
+        else
+            f_wrap_DVCState_with_Outputs(process, getEmptyOuputs())
+    }
+
     function f_resend_block_share(
         process: DVCState
     ): DVCStateAndOuputs
@@ -680,8 +716,8 @@ module DVC_Block_Proposer_Spec_Instr {
             state := process,
             outputs := getEmptyOuputs().(
                 block_shares_sent :=
-                    if process.block_shares_to_broadcast.Keys != {} then
-                        multicast_multiple(process.block_shares_to_broadcast.Values, process.peers)                        
+                    if process.signed_beacon_blocks_to_broadcast.Keys != {} then
+                        multicast_multiple(process.signed_beacon_blocks_to_broadcast.Values, process.peers)                        
                     else
                         {}
                     )
@@ -695,7 +731,7 @@ module DVC_Block_Proposer_Spec_Instr {
         DVCStateAndOuputs(
             state := process,
             outputs := getEmptyOuputs().(
-                randao_shares_sent :=
+                sent_randao_shares :=
                     if process.randao_shares_to_broadcast.Keys != {} then
                         multicast_multiple(process.randao_shares_to_broadcast.Values, process.peers)                        
                     else
@@ -704,4 +740,3 @@ module DVC_Block_Proposer_Spec_Instr {
         )
     }      
 }
-
