src/proofs/implementation_refinement/attestation_creation/dvc_spec_spec_instr_on_blocks_refinement.dfy
@@ -1,0 +1,336 @@
+include "../../../common/block_proposer/block_types.dfy"
+include "../../../common/block_proposer/block_common_functions.dfy"
+include "../../../common/block_proposer/block_signing_functions.dfy"
+include "../../../proofs/no_slashable_blocks/common/block_dvc_spec_axioms.dfy"
+include "../../../proofs/no_slashable_blocks/common/dvc_block_proposer_instrumented.dfy"
+include "../../../specs/dvc/dvc_block_proposer.dfy"
+include "../../../common/commons.dfy"
+include "../../no_slashable_blocks/common/block_dvc_spec_axioms.dfy"
+
+
+include "../../common/helper_pred_fcn.dfy"
+
+module Spec_Spec_NonInstr_Refinement
+{
+    import opened Block_Types 
+    import opened Block_Common_Functions
+    import opened Block_Signing_Functions    
+    import opened DVC_Block_Proposer_Spec_Axioms
+    import DVC_Block_Proposer_Spec_NonInstr
+    import DVC_Block_Proposer_Spec_Instr
+    import opened Helper_Pred_Fcn
+
+
+    predicate consensusEngineStateRel(
+        cei: DVC_Block_Proposer_Spec_Instr.BlockConsensusEngineState,
+        ceni: DVC_Block_Proposer_Spec_NonInstr.BlockConsensusEngineState
+    )
+    {
+        cei.active_consensus_instances_on_beacon_blocks == ceni.active_consensus_instances_on_beacon_blocks
+    }
+
+    predicate DVCStateRel(
+        dvci: DVC_Block_Proposer_Spec_Instr.DVCState,
+        dvcni: DVC_Block_Proposer_Spec_NonInstr.DVCState
+    )
+    {
+        && dvci.current_proposer_duty == dvcni.current_proposer_duty
+        && dvci.latest_proposer_duty == dvcni.latest_proposer_duty
+        && dvci.block_slashing_db == dvcni.block_slashing_db
+        && dvci.rcvd_randao_shares == dvcni.rcvd_randao_shares
+        && dvci.rcvd_signed_beacon_blocks == dvcni.rcvd_signed_beacon_blocks
+        && dvci.construct_complete_signed_randao_reveal == dvcni.construct_complete_signed_randao_reveal
+        && dvci.construct_complete_signed_block == dvcni.construct_complete_signed_block
+        && dvci.randao_shares_to_broadcast == dvcni.randao_shares_to_broadcast
+        && dvci.signed_beacon_blocks_to_broadcast == dvcni.signed_beacon_blocks_to_broadcast
+        && dvci.peers == dvcni.peers
+        && dvci.dv_pubkey == dvcni.dv_pubkey
+        && dvci.future_consensus_instances_on_blocks_already_decided == dvcni.future_consensus_instances_on_blocks_already_decided
+        && dvci.bn == dvcni.bn
+        && dvci.rs == dvcni.rs
+        && consensusEngineStateRel(dvci.block_consensus_engine_state, dvcni.block_consensus_engine_state)
+    }
+
+    predicate DVCStateAndOuputsRel(
+        dvcandoi: DVC_Block_Proposer_Spec_Instr.DVCStateAndOuputs,
+        dvcandoni: DVC_Block_Proposer_Spec_NonInstr.DVCStateAndOuputs        
+    )
+    {
+        && DVCStateRel(dvcandoi.state, dvcandoni.state)
+        && dvcandoi.outputs == dvcandoni.outputs
+    }
+
+    lemma refine_init(
+        dvci: DVC_Block_Proposer_Spec_Instr.DVCState,
+        dvcni: DVC_Block_Proposer_Spec_NonInstr.DVCState,
+        dv_pubkey: BLSPubkey,
+        peers: set<BLSPubkey>,                    
+        construct_complete_signed_randao_reveal: (set<BLSSignature>) -> Optional<BLSSignature>,
+        construct_complete_signed_block: (set<SignedBeaconBlock>) -> Optional<SignedBeaconBlock>,        
+        initial_block_slashing_db: set<SlashingDBBlock>,
+        rs_pubkey: BLSPubkey
+    )
+    requires DVC_Block_Proposer_Spec_Instr.Init.requires(
+                dvci, 
+                dv_pubkey,
+                peers,
+                construct_complete_signed_randao_reveal,
+                construct_complete_signed_block, 
+                initial_block_slashing_db,
+                rs_pubkey
+            )
+    requires DVC_Block_Proposer_Spec_Instr.Init(
+                dvci, 
+                dv_pubkey,
+                peers,
+                construct_complete_signed_randao_reveal,
+                construct_complete_signed_block, 
+                initial_block_slashing_db,
+                rs_pubkey
+            )
+    requires DVC_Block_Proposer_Spec_NonInstr.Init.requires(
+                dvcni, 
+                dv_pubkey,
+                peers,
+                construct_complete_signed_randao_reveal,
+                construct_complete_signed_block, 
+                initial_block_slashing_db,
+                rs_pubkey
+            )
+    requires DVC_Block_Proposer_Spec_NonInstr.Init(
+                dvcni, 
+                dv_pubkey,
+                peers,
+                construct_complete_signed_randao_reveal,
+                construct_complete_signed_block, 
+                initial_block_slashing_db,
+                rs_pubkey
+            )
+    ensures && var  dvcoi := 
+                    DVC_Block_Proposer_Spec_Instr.DVCStateAndOuputs(
+                        dvci,
+                        DVC_Block_Proposer_Spec_Instr.getEmptyOuputs()
+                    );
+            && var  dvconi := 
+                    DVC_Block_Proposer_Spec_NonInstr.DVCStateAndOuputs(
+                        dvcni,
+                        DVC_Block_Proposer_Spec_NonInstr.getEmptyOuputs()
+                    );
+            && DVCStateAndOuputsRel(dvcoi, dvconi);    
+    { }
+
+    lemma refine_f_terminate_current_proposer_duty(
+        dvci: DVC_Block_Proposer_Spec_Instr.DVCState,
+        dvcni: DVC_Block_Proposer_Spec_NonInstr.DVCState
+    )
+    requires DVC_Block_Proposer_Spec_Instr.f_terminate_current_proposer_duty.requires(dvci)
+    requires DVCStateRel(dvci, dvcni)
+    ensures DVC_Block_Proposer_Spec_NonInstr.f_terminate_current_proposer_duty.requires(dvcni)
+    ensures DVCStateRel(
+        DVC_Block_Proposer_Spec_Instr.f_terminate_current_proposer_duty(dvci), 
+        DVC_Block_Proposer_Spec_NonInstr.f_terminate_current_proposer_duty(dvcni)
+    ); 
+    {
+        if dvci.current_proposer_duty.isPresent()
+        {
+            var dvci_new :=
+                    dvci.(
+                        current_proposer_duty := None,
+                        block_consensus_engine_state := DVC_Block_Proposer_Spec_Instr.stopBlockConsensusInstances(
+                                        dvci.block_consensus_engine_state,
+                                        {dvci.current_proposer_duty.safe_get().slot}
+                        )               
+                    );                    
+            
+            assert dvcni.current_proposer_duty.isPresent();
+
+            var dvcni_new :=
+                    dvcni.(
+                        current_proposer_duty := None,
+                        block_consensus_engine_state := DVC_Block_Proposer_Spec_NonInstr.stopBlockConsensusInstances(
+                                        dvcni.block_consensus_engine_state,
+                                        {dvcni.current_proposer_duty.safe_get().slot}
+                        )               
+                    );
+
+            assert  DVCStateRel(dvci_new, dvcni_new); 
+        }
+    }  
+
+    lemma refine_f_serve_proposer_duty(
+        dvci: DVC_Block_Proposer_Spec_Instr.DVCState,
+        dvcni: DVC_Block_Proposer_Spec_NonInstr.DVCState,
+        proposer_duty: ProposerDuty
+    )
+    requires DVC_Block_Proposer_Spec_Instr.f_serve_proposer_duty.requires(dvci, proposer_duty)
+    requires DVCStateRel(dvci, dvcni)
+    ensures DVC_Block_Proposer_Spec_NonInstr.f_serve_proposer_duty.requires(dvcni, proposer_duty)
+    ensures DVCStateAndOuputsRel(
+        DVC_Block_Proposer_Spec_Instr.f_serve_proposer_duty(dvci, proposer_duty), 
+        DVC_Block_Proposer_Spec_NonInstr.f_serve_proposer_duty(dvcni, proposer_duty)
+    );    
+    { }
+
+    lemma refine_f_broadcast_randao_share(
+        dvci: DVC_Block_Proposer_Spec_Instr.DVCState,
+        dvcni: DVC_Block_Proposer_Spec_NonInstr.DVCState,
+        proposer_duty: ProposerDuty
+    )
+    requires DVC_Block_Proposer_Spec_Instr.f_broadcast_randao_share.requires(dvci, proposer_duty)
+    requires DVCStateRel(dvci, dvcni)
+    ensures DVC_Block_Proposer_Spec_NonInstr.f_broadcast_randao_share.requires(dvcni, proposer_duty)
+    ensures DVCStateAndOuputsRel(
+        DVC_Block_Proposer_Spec_Instr.f_broadcast_randao_share(dvci, proposer_duty), 
+        DVC_Block_Proposer_Spec_NonInstr.f_broadcast_randao_share(dvcni, proposer_duty)
+    );    
+    { }
+
+    lemma refine_f_check_for_next_duty(
+        dvci: DVC_Block_Proposer_Spec_Instr.DVCState,
+        dvcni: DVC_Block_Proposer_Spec_NonInstr.DVCState,
+        proposer_duty: ProposerDuty
+    )
+    requires DVC_Block_Proposer_Spec_Instr.f_check_for_next_duty.requires(dvci, proposer_duty)
+    requires DVCStateRel(dvci, dvcni)
+    ensures DVC_Block_Proposer_Spec_NonInstr.f_check_for_next_duty.requires(dvcni, proposer_duty)
+    ensures DVCStateAndOuputsRel(
+        DVC_Block_Proposer_Spec_Instr.f_check_for_next_duty(dvci, proposer_duty), 
+        DVC_Block_Proposer_Spec_NonInstr.f_check_for_next_duty(dvcni, proposer_duty)
+    )    
+    {
+        var slot := proposer_duty.slot;
+        if slot in dvci.future_consensus_instances_on_blocks_already_decided.Keys
+        { }
+        else
+        { }
+    }
+
+    lemma refine_f_listen_for_randao_shares(
+        dvci: DVC_Block_Proposer_Spec_Instr.DVCState,
+        dvcni: DVC_Block_Proposer_Spec_NonInstr.DVCState,
+        randao_share: RandaoShare
+    )
+    requires DVC_Block_Proposer_Spec_Instr.f_listen_for_randao_shares.requires(dvci, randao_share)
+    requires DVCStateRel(dvci, dvcni)
+    ensures DVC_Block_Proposer_Spec_NonInstr.f_listen_for_randao_shares.requires(dvcni, randao_share)
+    ensures DVCStateAndOuputsRel(
+        DVC_Block_Proposer_Spec_Instr.f_listen_for_randao_shares(dvci, randao_share), 
+        DVC_Block_Proposer_Spec_NonInstr.f_listen_for_randao_shares(dvcni, randao_share)
+    );    
+    { }
+
+    lemma refine_f_start_consensus_if_can_construct_randao_share(
+        dvci: DVC_Block_Proposer_Spec_Instr.DVCState,
+        dvcni: DVC_Block_Proposer_Spec_NonInstr.DVCState
+    )
+    requires DVC_Block_Proposer_Spec_Instr.f_start_consensus_if_can_construct_randao_share.requires(dvci)
+    requires DVCStateRel(dvci, dvcni)
+    ensures DVC_Block_Proposer_Spec_NonInstr.f_start_consensus_if_can_construct_randao_share.requires(dvcni)
+    ensures DVCStateAndOuputsRel(
+        DVC_Block_Proposer_Spec_Instr.f_start_consensus_if_can_construct_randao_share(dvci), 
+        DVC_Block_Proposer_Spec_NonInstr.f_start_consensus_if_can_construct_randao_share(dvcni)
+    );    
+    { }
+
+    lemma refine_f_block_consensus_decided(
+        dvci: DVC_Block_Proposer_Spec_Instr.DVCState,
+        dvcni: DVC_Block_Proposer_Spec_NonInstr.DVCState,
+        id: Slot,
+        block: BeaconBlock
+    )
+    requires DVC_Block_Proposer_Spec_Instr.f_block_consensus_decided.requires(dvci, id, block)
+    requires DVCStateRel(dvci, dvcni)
+    ensures DVC_Block_Proposer_Spec_NonInstr.f_block_consensus_decided.requires(dvcni, id, block)
+    ensures DVCStateAndOuputsRel(
+        DVC_Block_Proposer_Spec_Instr.f_block_consensus_decided(dvci, id, block), 
+        DVC_Block_Proposer_Spec_NonInstr.f_block_consensus_decided(dvcni, id, block)
+    );       
+    { }
+
+    lemma refine_f_listen_for_block_signature_shares(
+        dvci: DVC_Block_Proposer_Spec_Instr.DVCState,
+        dvcni: DVC_Block_Proposer_Spec_NonInstr.DVCState,
+        block_share: SignedBeaconBlock
+    )
+    requires DVC_Block_Proposer_Spec_Instr.f_listen_for_block_signature_shares.requires(dvci, block_share)
+    requires DVCStateRel(dvci, dvcni)
+    ensures DVC_Block_Proposer_Spec_NonInstr.f_listen_for_block_signature_shares.requires(dvcni, block_share)
+    ensures DVCStateAndOuputsRel(
+        DVC_Block_Proposer_Spec_Instr.f_listen_for_block_signature_shares(dvci, block_share), 
+        DVC_Block_Proposer_Spec_NonInstr.f_listen_for_block_signature_shares(dvcni, block_share)
+    );    
+    { }     
+
+    
+
+    lemma refine_f_listen_for_new_imported_blocks(
+        dvci: DVC_Block_Proposer_Spec_Instr.DVCState,
+        dvcni: DVC_Block_Proposer_Spec_NonInstr.DVCState,
+        block: BeaconBlock
+    )
+    requires DVC_Block_Proposer_Spec_Instr.f_listen_for_new_imported_blocks.requires(dvci, block)
+    requires DVCStateRel(dvci, dvcni)
+    ensures DVC_Block_Proposer_Spec_NonInstr.f_listen_for_new_imported_blocks.requires(dvcni, block)
+    ensures DVCStateAndOuputsRel(
+        DVC_Block_Proposer_Spec_Instr.f_listen_for_new_imported_blocks(dvci, block), 
+        DVC_Block_Proposer_Spec_NonInstr.f_listen_for_new_imported_blocks(dvcni, block)
+    );     
+    { }
+
+    lemma refine_f_resend_randao_share(
+        dvci: DVC_Block_Proposer_Spec_Instr.DVCState,
+        dvcni: DVC_Block_Proposer_Spec_NonInstr.DVCState
+    )
+    requires DVC_Block_Proposer_Spec_Instr.f_resend_randao_share.requires(dvci)
+    requires DVCStateRel(dvci, dvcni)
+    ensures DVC_Block_Proposer_Spec_NonInstr.f_resend_randao_share.requires(dvcni)
+    ensures DVCStateAndOuputsRel(
+        DVC_Block_Proposer_Spec_Instr.f_resend_randao_share(dvci), 
+        DVC_Block_Proposer_Spec_NonInstr.f_resend_randao_share(dvcni)
+    ); 
+    { }
+
+    lemma refine_f_resend_block_share(
+        dvci: DVC_Block_Proposer_Spec_Instr.DVCState,
+        dvcni: DVC_Block_Proposer_Spec_NonInstr.DVCState
+    )
+    requires DVC_Block_Proposer_Spec_Instr.f_resend_block_share.requires(dvci)
+    requires DVCStateRel(dvci, dvcni)
+    ensures DVC_Block_Proposer_Spec_NonInstr.f_resend_block_share.requires(dvcni)
+    ensures DVCStateAndOuputsRel(
+        DVC_Block_Proposer_Spec_Instr.f_resend_block_share(dvci), 
+        DVC_Block_Proposer_Spec_NonInstr.f_resend_block_share(dvcni)
+    ); 
+    { }
+
+    lemma refine_f_process_event(
+        dvci: DVC_Block_Proposer_Spec_Instr.DVCState,
+        dvcni: DVC_Block_Proposer_Spec_NonInstr.DVCState,
+        event: Event
+    )
+    requires DVC_Block_Proposer_Spec_Instr.f_process_event.requires(dvci, event)
+    requires DVCStateRel(dvci, dvcni)
+    ensures DVC_Block_Proposer_Spec_NonInstr.f_process_event.requires(dvcni, event)
+    ensures DVCStateAndOuputsRel(
+        DVC_Block_Proposer_Spec_Instr.f_process_event(dvci, event), 
+        DVC_Block_Proposer_Spec_NonInstr.f_process_event(dvcni, event)
+    ); 
+    {
+        match event 
+            case ServeProposerDuty(proposer_duty) => 
+                refine_f_serve_proposer_duty(dvci, dvcni, proposer_duty);
+            case BlockConsensusDecided(id, block) => 
+                refine_f_block_consensus_decided(dvci, dvcni, id,  block);
+            case ReceiveRandaoShare(randao_share) => 
+                refine_f_listen_for_randao_shares(dvci, dvcni, randao_share);
+            case ReceiveSignedBeaconBlock(block_share) => 
+                refine_f_listen_for_block_signature_shares(dvci, dvcni, block_share);
+            case ImportedNewBlock(block) => 
+                refine_f_listen_for_new_imported_blocks(dvci, dvcni, block);
+            case ResendRandaoRevealSignatureShare => 
+                refine_f_resend_randao_share(dvci, dvcni);
+            case ResendBlockShare => 
+                refine_f_resend_block_share(dvci, dvcni);
+            case NoEvent => 
+    }    
+}
